Working on ADT refinement with

ADT.v
@@ -8,47 +8,58 @@ Local Open Scope type_scope.
 
 (** * Basic ADT definitions *)
 (** Type of a context *)
-Definition Build_ADTContext (rep mutIdx obsIdx : Type) : Context :=
+Definition Build_ADTContext
+           (rep mutIdx obsIdx : Type)
+           (mutDom : mutIdx -> Type)
+           (obsDom obsCod : obsIdx -> Type): Context :=
   {| names := mutIdx + obsIdx;
-     dom idx := rep * nat;
+     dom idx := rep *
+                match idx with
+                  | inl mIdx => mutDom mIdx
+                  | inr oIdx => obsDom oIdx
+                end;
      cod idx := match idx with
                   | inl mIdx => rep
-                  | inr oIdx => nat
+                  | inr oIdx => obsCod oIdx
                 end |}.
 
 (** Type of a mutator method *)
-Definition mutatorMethodTypeUnbundled (Ty mutIdx obsIdx : Type)
+Definition mutatorMethodTypeUnbundled (Ty mutIdx obsIdx dom : Type)
+           (mutDom : mutIdx -> Type)
+           (obsDom obsCod : obsIdx -> Type)
            (* we give a [Context] here so typeclass resolution can pick it up *)
-           (ctx := Build_ADTContext Ty mutIdx obsIdx)
+           (ctx := Build_ADTContext Ty mutDom obsDom obsCod)
   := Ty    (* Initial model *)
-     -> nat (* Actual argument*)
+     -> dom (* Actual argument*)
      -> Comp Ty (* Final Model *).
 
 (** Type of an obeserver method *)
-Definition observerMethodTypeUnbundled (Ty mutIdx obsIdx : Type)
+Definition observerMethodTypeUnbundled (Ty mutIdx obsIdx dom cod : Type)
+           (mutDom : mutIdx -> Type)
+           (obsDom obsCod : obsIdx -> Type)
            (* we give a [Context] here so typeclass resolution can pick it up *)
-           (ctx := Build_ADTContext Ty mutIdx obsIdx)
+           (ctx := Build_ADTContext Ty mutDom obsDom obsCod)
   := Ty    (* Initial model *)
-     -> nat (* Actual argument*)
-     -> Comp nat. (* Return value *)
+     -> dom (* Actual argument*)
+     -> Comp cod. (* Return value *)
 
 (** Type of a mutator method bundled with its context *)
-Definition mutatorMethodType (Ty : Type)
+Definition mutatorMethodType (Ty dom : Type)
   := Ty    (* Initial model *)
-     -> nat (* Actual argument*)
+     -> dom (* Actual argument*)
      -> BundledComp Ty (* Final Model *).
 
 (** Type of an obeserver method *)
-Definition observerMethodType (Ty : Type)
+Definition observerMethodType (Ty dom cod : Type)
   := Ty    (* Initial model *)
-     -> nat (* Actual argument*)
-     -> BundledComp nat. (* Return value *)
+     -> dom (* Actual argument*)
+     -> BundledComp cod. (* Return value *)
 
 (** Interface of an ADT *)
 Record ADT :=
   {
     Rep : Type;
-    (** The way we model state mathematically *)
+    (** The representation type of the ADT **)
 
     MutatorIndex : Type;
     (** The index set of mutators *)
@@ -56,16 +67,28 @@ Record ADT :=
     ObserverIndex : Type;
     (** The index set of observers *)
 
-    UnbundledMutatorMethods : MutatorIndex -> mutatorMethodTypeUnbundled Rep MutatorIndex ObserverIndex;
+    MutatorDom : MutatorIndex -> Type;
+
+    ObserverDom : ObserverIndex -> Type;
+
+    ObserverCod : ObserverIndex -> Type;
+
+    UnbundledMutatorMethods :
+      forall idx : MutatorIndex,
+        mutatorMethodTypeUnbundled Rep (MutatorDom idx)
+                                   MutatorDom ObserverDom ObserverCod;
     (** Mutator method implementations *)
 
-    UnbundledObserverMethods : ObserverIndex -> observerMethodTypeUnbundled Rep MutatorIndex ObserverIndex
+    UnbundledObserverMethods :
+      forall idx : ObserverIndex,
+        observerMethodTypeUnbundled Rep (ObserverDom idx) (ObserverCod idx)
+                                    MutatorDom ObserverDom ObserverCod
     (** Observer method implementations *)
 
   }.
 
 Definition ADTLookupContext (A : ADT) : LookupContext
-  := {| LContext := Build_ADTContext (Rep A) (MutatorIndex A) (ObserverIndex A);
+  := {| LContext := Build_ADTContext (Rep A) (MutatorDom A) (ObserverDom A) (ObserverCod A);
         lookup idx := match idx with
                         | inl mIdx => fun state_value =>
                                         UnbundledMutatorMethods A mIdx (fst state_value) (snd state_value)
@@ -73,7 +96,10 @@ Definition ADTLookupContext (A : ADT) : LookupContext
                                         UnbundledObserverMethods A oIdx (fst state_value) (snd state_value)
                       end |}.
 
-Definition MutatorMethods (A : ADT) (i : MutatorIndex A) : mutatorMethodType (Rep A)
-  := fun m x => ``[ UnbundledMutatorMethods A i m x with ADTLookupContext A ]``.
-Definition ObserverMethods (A : ADT) (i : ObserverIndex A) : observerMethodType (Rep A)
+Definition MutatorMethods (A : ADT) (i : MutatorIndex A)
+: mutatorMethodType (Rep A) (MutatorDom A i)
+  := fun m x => ``[ UnbundledMutatorMethods A i m x with ADTLookupContext A ]`` .
+
+Definition ObserverMethods (A : ADT) (i : ObserverIndex A)
+: observerMethodType (Rep A) (ObserverDom A i) (ObserverCod A i)
   := fun m x => ``[ UnbundledObserverMethods A i m x with ADTLookupContext A ]``.
