Makefile
@@ -60,7 +60,7 @@ html: Makefile.coq
 #	@echo
 
 Makefile.coq: Makefile $(VS)
-	coq_makefile $(VS) COQC = " $(SILENCE_COQC)\$$(TIMER) \"\$$(COQBIN)coqc\"" COQDEP = " $(SILENCE_COQDEP)\"\$$(COQBIN)coqdep\" -c" COQDOCFLAGS = "$(COQDOCFLAGS)" -arg -dont-load-proofs -R . ADTSynthesis -o Makefile.coq
+	coq_makefile $(VS) COQC = " $(SILENCE_COQC)\$$(TIMER) \"\$$(COQBIN)coqc\"" COQDEP = " $(SILENCE_COQDEP)\"\$$(COQBIN)coqdep\" -c" COQDOCFLAGS = "$(COQDOCFLAGS)" -arg -dont-load-proofs -R Computation Computation -o Makefile.coq
 
 clean:: Makefile.coq
 	$(MAKE) -f Makefile.coq clean
